src/Std/Tactic/BVDecide/LRAT/Internal/CNF.lean
@@ -6,6 +6,8 @@ Authors: Josh Clune
 prelude
 import Std.Tactic.BVDecide.LRAT.Internal.Formula.Class
 
+set_option grind.warning false
+
 namespace Std.Tactic.BVDecide
 namespace LRAT
 namespace Internal
@@ -14,18 +16,10 @@ open Clause Formula Std Sat
 
 namespace Literal
 
-theorem sat_iff (p : α → Bool) (a : α) (b : Bool) : p ⊨ (a, b) ↔ (p a) = b := by
-  simp only [Entails.eval]
+theorem sat_iff (p : α → Bool) (a : α) (b : Bool) : p ⊨ (a, b) ↔ (p a) = b := Iff.rfl
 
 theorem sat_negate_iff_not_sat {p : α → Bool} {l : Literal α} : p ⊨ Literal.negate l ↔ p ⊭ l := by
-  simp only [Literal.negate, sat_iff]
-  constructor
-  · intro h pl
-    rw [sat_iff, h] at pl
-    simp at pl
-  · intro h
-    rw [sat_iff] at h
-    cases h : p l.fst <;> simp_all
+  grind [Literal.negate, sat_iff, cases Bool]
 
 theorem unsat_of_limplies_complement [Entails α t] (x : t) (l : Literal α) :
     Limplies α x l → Limplies α x (Literal.negate l) → Unsatisfiable α x := by
@@ -41,7 +35,7 @@ namespace Clause
 
 theorem sat_iff_exists [Clause α β] (p : α → Bool) (c : β) : p ⊨ c ↔ ∃ l ∈ toList c, p ⊨ l := by
   simp only [(· ⊨ ·), eval]
-  simp only [List.any_eq_true, decide_eq_true_eq, Prod.exists, Bool.exists_bool]
+  grind [List.any_eq_true]
 
 theorem limplies_iff_mem [DecidableEq α] [Clause α β] (l : Literal α) (c : β) :
     Limplies α l c ↔ l ∈ toList c := by
@@ -53,49 +47,19 @@ theorem limplies_iff_mem [DecidableEq α] [Clause α β] (l : Literal α) (c : �
     have pl : p ⊨ l := by simp only [(· ⊨ ·), ite_true, p]
     specialize h p pl
     rcases h with ⟨v, ⟨h1, h2⟩ | ⟨h1, h2⟩⟩
+    · simp only [(· ⊨ ·)] at h2
+      grind
     · simp only [(· ⊨ ·), p] at h2
       split at h2
-      · next v_eq_l =>
-        cases l
-        simp_all
-      · next v_ne_l =>
-        simp only [decide_eq_false_iff_not] at h2
-        exfalso
-        exact h2 h1
-    · simp only [(· ⊨ ·), p] at h2
-      split at h2
-      · next v_eq_l =>
-        cases l
-        simp_all
-      · next v_ne_l =>
-        simp only [decide_eq_true_eq] at h2
-        exfalso
-        rcases not_tautology c (v, true) with v_not_in_c | negv_not_in_c
-        · exact v_not_in_c h1
-        · simp only [Literal.negate, Bool.not_true] at negv_not_in_c
-          exact negv_not_in_c h2
-  · intro h p pl
-    apply Exists.intro l.1
-    by_cases hl : l.2
-    · apply Or.inr
-      rw [← hl]
-      exact ⟨h, pl⟩
-    · apply Or.inl
-      simp only [Bool.not_eq_true] at hl
-      rw [← hl]
-      exact ⟨h, pl⟩
+      · grind
+      · rcases not_tautology c (v, true) <;> grind [Literal.negate]
+  · grind [cases Bool]
 
 theorem entails_of_entails_delete [DecidableEq α] [Clause α β] {p : α → Bool} {c : β}
     {l : Literal α} :
     p ⊨ delete c l → p ⊨ c := by
-  intro h
-  simp only [(· ⊨ ·), eval, List.any_eq_true, decide_eq_true_eq, Prod.exists, Bool.exists_bool] at h
-  simp only [(· ⊨ ·), eval, List.any_eq_true, decide_eq_true_eq, Prod.exists, Bool.exists_bool]
-  rcases h with ⟨v, ⟨h1, h2⟩ | ⟨h1, h2⟩⟩
-  · simp only [delete_iff, ne_eq] at h1
-    exact Exists.intro v <| Or.inl ⟨h1.2, h2⟩
-  · simp only [delete_iff, ne_eq] at h1
-    exact Exists.intro v <| Or.inr ⟨h1.2, h2⟩
+  simp only [(· ⊨ ·), eval] at ⊢
+  grind [delete_iff, List.any_eq_true]
 
 end Clause
 
@@ -103,27 +67,22 @@ namespace Formula
 
 theorem sat_iff_forall [Clause α β] [Entails α σ] [Formula α β σ] (p : α → Bool) (f : σ) :
     p ⊨ f ↔ ∀ c : β, c ∈ toList f → p ⊨ c := by
-  simp only [(· ⊨ ·), formulaEntails_def p f]
-  simp only [List.all_eq_true, decide_eq_true_eq]
+  simp only [formulaEntails_def]
+  grind [List.all_eq_true]
 
 theorem limplies_insert [Clause α β] [Entails α σ] [Formula α β σ] {c : β} {f : σ} :
     Limplies α (insert f c) f := by
   intro p
   simp only [formulaEntails_def, List.all_eq_true, decide_eq_true_eq]
   intro h c' c'_in_f
-  have c'_in_fc : c' ∈ toList (insert f c) := by
-    simp only [insert_iff, List.toList_toArray, List.mem_singleton]
-    exact Or.inr c'_in_f
-  exact h c' c'_in_fc
+  have c'_in_fc : c' ∈ toList (insert f c) := by grind [insert_iff]
+  grind
 
 theorem limplies_delete [Clause α β] [Entails α σ] [Formula α β σ] {f : σ} {arr : Array Nat} :
     Limplies α f (delete f arr) := by
   intro p
-  simp only [formulaEntails_def, List.all_eq_true, decide_eq_true_eq]
-  intro h c c_in_f_del
-  have del_f_subset := delete_subset f arr
-  specialize del_f_subset c c_in_f_del
-  exact h c del_f_subset
+  simp only [formulaEntails_def]
+  grind [List.all_eq_true, delete_subset]
 
 end Formula
 
