src/Std/Tactic/BVDecide/LRAT/Internal/Formula/Lemmas.lean
@@ -7,6 +7,11 @@ prelude
 import Std.Tactic.BVDecide.LRAT.Internal.Formula.Implementation
 import Std.Tactic.BVDecide.LRAT.Internal.CNF
 
+set_option grind.warning false -- I've only made a minimal effort to use grind here so far.
+
+-- FIXME: move these to the library.
+attribute [local grind] Array.size_modify Array.getElem_modify
+
 /-!
 This module contains basic statements about the invariants that are satisfied by the LRAT checker
 implementation in `Implementation`.
@@ -20,6 +25,8 @@ namespace DefaultFormula
 
 open Std.Sat
 open DefaultClause DefaultFormula Assignment
+
+attribute [local grind] insert ofArray
 
 /--
 This invariant states that if the `assignments` field of a default formula `f` indicates that `f`
@@ -86,25 +93,23 @@ def ReadyForRatAdd {n : Nat} (f : DefaultFormula n) : Prop := f.ratUnits = #[] �
 theorem rupUnits_insert {n : Nat} (f : DefaultFormula n) (c : DefaultClause n) :
     (insert f c).rupUnits = f.rupUnits := by
   simp only [insert]
-  split <;> simp only
+  grind
 
 theorem ratUnits_insert {n : Nat} (f : DefaultFormula n) (c : DefaultClause n) :
     (insert f c).ratUnits = f.ratUnits := by
   simp only [insert]
-  split <;> simp only
+  grind
 
 theorem size_ofArray_fold_fn {n : Nat} (assignments : Array Assignment)
     (cOpt : Option (DefaultClause n)) :
     (ofArray_fold_fn assignments cOpt).size = assignments.size := by
   rw [ofArray_fold_fn.eq_def]
-  split
-  · rfl
-  · split <;> simp [Array.size_modify]
+  grind
 
 theorem readyForRupAdd_ofArray {n : Nat} (arr : Array (Option (DefaultClause n))) :
     ReadyForRupAdd (ofArray arr) := by
   constructor
-  · simp only [ofArray]
+  · grind
   · have hsize : (ofArray arr).assignments.size = n := by
       simp only [ofArray, ← Array.foldl_toList]
       have hb : (Array.replicate n unassigned).size = n := by simp only [Array.size_replicate]
@@ -172,7 +177,7 @@ theorem readyForRupAdd_ofArray {n : Nat} (arr : Array (Option (DefaultClause n))
               specialize ih l true
               simp only [hasAssignment, ite_false] at ih
               rw [b_eq_true, Subtype.ext i_eq_l]
-              exact ih h
+              grind
             · next b_eq_false =>
               rw [isUnit_iff, DefaultClause.toList] at heq
               simp only [toList, ofArray, List.map, List.append_nil, List.mem_filterMap, id_eq, exists_eq_right]
@@ -180,20 +185,15 @@ theorem readyForRupAdd_ofArray {n : Nat} (arr : Array (Option (DefaultClause n))
               simp only [unit, b_eq_false, i_eq_l]
               have c_def : c = ⟨c.clause, c.nodupkey, c.nodup⟩ := rfl
               simp only [heq] at c_def
-              rw [c_def] at cOpt_in_arr
-              exact cOpt_in_arr
-          · next i_ne_l =>
-            simp only [Array.getElem_modify_of_ne (Ne.symm i_ne_l)] at h
-            exact ih i b h
+              grind
+          · next i_ne_l => grind
     rcases List.foldlRecOn arr.toList ofArray_fold_fn hb hl with ⟨_h_size, h'⟩
-    intro i b h
-    simp only [ofArray, ← Array.foldl_toList] at h
-    exact h' i b h
+    grind [ofArray]
 
 theorem readyForRatAdd_ofArray {n : Nat} (arr : Array (Option (DefaultClause n))) :
     ReadyForRatAdd (ofArray arr) := by
   constructor
-  · simp only [ofArray]
+  · grind
   · exact readyForRupAdd_ofArray arr
 
 theorem insert_iff {n : Nat} (f : DefaultFormula n) (c1 : DefaultClause n) (c2 : DefaultClause n) :
@@ -203,57 +203,39 @@ theorem insert_iff {n : Nat} (f : DefaultFormula n) (c1 : DefaultClause n) (c2 :
   by_cases c2 = c1
   · next c2_eq_c1 =>
     constructor
-    · intro _
-      exact Or.inl c2_eq_c1
+    · grind
     · intro _
       apply Or.inl
       simp only [c2_eq_c1, insert]
-      split <;> simp
+      grind
   · next c2_ne_c1 =>
     constructor
     · intro h
-      apply Or.inr
       rcases h with h | h | h
-      · apply Or.inl
-        simp only [insert] at h
-        split at h
-        all_goals
-          simp only [Array.toList_push, List.mem_append, List.mem_singleton, Option.some.injEq] at h
-          rcases h with h | h
-          · exact h
-          · exact False.elim <| c2_ne_c1 h
-      · rw [rupUnits_insert] at h
-        exact Or.inr <| Or.inl h
-      · rw [ratUnits_insert] at h
-        exact Or.inr <| Or.inr h
+      · simp only [insert] at h
+        grind
+      · grind [rupUnits_insert]
+      · grind [ratUnits_insert]
     · intro h
       rcases h with h | h | h | h
-      · exact False.elim <| c2_ne_c1 h
-      · apply Or.inl
-        simp only [insert]
-        split
-        all_goals
-          simp only [Array.toList_push, List.mem_append, List.mem_singleton, Option.some.injEq]
-          exact Or.inl h
-      · rw [rupUnits_insert]
-        exact Or.inr <| Or.inl h
-      · rw [ratUnits_insert]
-        exact Or.inr <| Or.inr h
+      · grind
+      · simp only [insert]
+        grind
+      · grind [rupUnits_insert]
+      · grind [ratUnits_insert]
 
 theorem limplies_insert {n : Nat} (f : DefaultFormula n) (c : DefaultClause n) :
     Limplies (PosFin n) (insert f c) f := by
   intro p
-  simp only [formulaEntails_def, List.all_eq_true, decide_eq_true_eq]
+  simp only [formulaEntails_def, List.all_eq_true]
   intro h c' c'_in_f
-  have c'_in_fc : c' ∈ toList (insert f c) := by
-    simp only [insert_iff, List.toList_toArray, List.mem_singleton]
-    exact Or.inr c'_in_f
-  exact h c' c'_in_fc
+  have c'_in_fc : c' ∈ toList (insert f c) := by grind [insert_iff]
+  grind
 
 theorem size_assignments_insert {n : Nat} (f : DefaultFormula n) (c : DefaultClause n) :
     (insert f c).assignments.size = f.assignments.size := by
   simp only [insert]
-  split <;> simp only [Array.size_modify]
+  grind
 
 theorem readyForRupAdd_insert {n : Nat} (f : DefaultFormula n) (c : DefaultClause n) :
     ReadyForRupAdd f → ReadyForRupAdd (insert f c) := by
@@ -267,9 +249,7 @@ theorem readyForRupAdd_insert {n : Nat} (f : DefaultFormula n) (c : DefaultClaus
       List.mem_map, Prod.exists, Bool.exists_bool] at hf
     simp only [toList, Array.toList_push, List.append_assoc, List.mem_append, List.mem_filterMap,
       List.mem_singleton, id_eq, exists_eq_right, Option.some.injEq, List.mem_map, Prod.exists, Bool.exists_bool]
-    rcases hf with hf | hf
-    · exact (Or.inl ∘ Or.inl) hf
-    · exact Or.inr hf
+    grind
   · next l hc =>
     have hsize : (Array.modify f.assignments l.1 addPosAssignment).size = n := by
       rw [Array.size_modify, f_readyForRupAdd.2.1]
@@ -307,9 +287,7 @@ theorem readyForRupAdd_insert {n : Nat} (f : DefaultFormula n) (c : DefaultClaus
         exists_eq_right, List.mem_map, Prod.exists, Bool.exists_bool] at hf
       simp only [toList, Array.toList_push, List.append_assoc, List.mem_append, List.mem_filterMap,
         List.mem_singleton, id_eq, exists_eq_right, Option.some.injEq, List.mem_map, Prod.exists, Bool.exists_bool]
-      rcases hf with hf | hf
-      · exact Or.inl <| Or.inl hf
-      · exact Or.inr hf
+      grind
   · next l hc =>
     have hsize : (Array.modify f.assignments l.1 addNegAssignment).size = n := by
       rw [Array.size_modify, f_readyForRupAdd.2.1]
@@ -337,23 +315,20 @@ theorem readyForRupAdd_insert {n : Nat} (f : DefaultFormula n) (c : DefaultClaus
               simp only [b_eq_false, Subtype.ext l_eq_i, not_true] at ib_ne_c
           simp only [hasAssignment, b_eq_false, l_eq_i, Array.getElem_modify_self, ite_true, hasPos_addNeg] at hb
           simp only [hasAssignment, b_eq_false, ite_true, hb]
-        · next l_ne_i =>
-          simp only [Array.getElem_modify_of_ne l_ne_i] at hb
-          exact hb
+        · next l_ne_i => grind
       specialize hf hb'
       simp only [toList, List.append_assoc, List.mem_append, List.mem_filterMap, id_eq,
         exists_eq_right, List.mem_map, Prod.exists, Bool.exists_bool] at hf
       simp only [toList, Array.toList_push, List.append_assoc, List.mem_append, List.mem_filterMap,
-        List.mem_singleton, id_eq, exists_eq_right, Option.some.injEq, List.mem_map, Prod.exists, Bool.exists_bool]
-      rcases hf with hf | hf
-      · exact Or.inl <| Or.inl hf
-      · exact Or.inr hf
+        List.mem_singleton, id_eq, exists_eq_right, Option.some.injEq, List.mem_map]
+      grind
 
 theorem readyForRatAdd_insert {n : Nat} (f : DefaultFormula n) (c : DefaultClause n) :
     ReadyForRatAdd f → ReadyForRatAdd (insert f c) := by
   intro h
   constructor
-  · simp only [insert, h.1] <;> split <;> rfl
+  · simp only [insert, h.1]
+    grind
   · exact readyForRupAdd_insert f c h.2
 
 theorem mem_of_insertRupUnits {n : Nat} (f : DefaultFormula n) (units : CNF.Clause (PosFin n))
@@ -363,36 +338,27 @@ theorem mem_of_insertRupUnits {n : Nat} (f : DefaultFormula n) (units : CNF.Clau
     List.mem_filterMap, id_eq, exists_eq_right, List.mem_map, Prod.exists, Bool.exists_bool]
   intro h
   have hb : ∀ l : Literal (PosFin n), l ∈ (f.rupUnits, f.assignments, false).1.toList → (l ∈ f.rupUnits.toList ∨ l ∈ units) := by
-    intro l hl
-    exact Or.inl hl
+    grind
   have hl (acc : Array (Literal (PosFin n)) × Array Assignment × Bool)
     (ih : ∀ l : Literal (PosFin n), l ∈ acc.1.toList → l ∈ f.rupUnits.toList ∨ l ∈ units)
     (unit : Literal (PosFin n)) (unit_in_units : unit ∈ units) :
     ∀ l : Literal (PosFin n), l ∈ (insertUnit acc unit).1.toList → (l ∈ f.rupUnits.toList ∨ l ∈ units) := by
     intro l hl
     rw [insertUnit.eq_def] at hl
-    dsimp at hl
-    split at hl
-    · exact ih l hl
-    · simp only [Array.toList_push, List.mem_append, List.mem_singleton] at hl
-      rcases hl with l_in_acc | l_eq_unit
-      · exact ih l l_in_acc
-      · rw [l_eq_unit]
-        exact Or.inr unit_in_units
+    grind
   have h_insertUnit_fold := List.foldlRecOn units insertUnit hb hl
   rcases h with h | ⟨i, ⟨h1, h2⟩ | ⟨h1, h2⟩⟩ | h
-  · exact Or.inr <| Or.inl h
+  · grind
   · rcases h_insertUnit_fold (i, false) h1 with h_insertUnit_fold | h_insertUnit_fold
     · apply Or.inr ∘ Or.inr ∘ Or.inl ∘ Exists.intro i ∘ Or.inl
-      exact ⟨h_insertUnit_fold, h2⟩
+      grind
     · apply Or.inl ∘ Exists.intro i ∘ Or.inl
       exact ⟨h_insertUnit_fold, h2⟩
   · rcases h_insertUnit_fold (i, true) h1 with h_insertUnit_fold | h_insertUnit_fold
-    · apply Or.inr ∘ Or.inr ∘ Or.inl ∘ Exists.intro i ∘ Or.inr
-      exact ⟨h_insertUnit_fold, h2⟩
+    · grind
     · apply Or.inl ∘ Exists.intro i ∘ Or.inr
       exact ⟨h_insertUnit_fold, h2⟩
-  · exact (Or.inr ∘ Or.inr ∘ Or.inr) h
+  · grind
 
 theorem mem_of_insertRatUnits {n : Nat} (f : DefaultFormula n) (units : CNF.Clause (PosFin n))
     (c : DefaultClause n) :
@@ -408,38 +374,29 @@ theorem mem_of_insertRatUnits {n : Nat} (f : DefaultFormula n) (units : CNF.Clau
     ∀ l : Literal (PosFin n), l ∈ (insertUnit acc unit).1.toList → (l ∈ f.ratUnits.toList ∨ l ∈ units) := by
     intro l hl
     rw [insertUnit.eq_def] at hl
-    dsimp at hl
-    split at hl
-    · exact ih l hl
-    · simp only [Array.toList_push, List.mem_append, List.mem_singleton] at hl
-      rcases hl with l_in_acc | l_eq_unit
-      · exact ih l l_in_acc
-      · rw [l_eq_unit]
-        exact Or.inr unit_in_units
+    grind
   have h_insertUnit_fold := List.foldlRecOn units insertUnit hb hl
   rcases h with h | h | ⟨i, ⟨h1, h2⟩ | ⟨h1, h2⟩⟩
-  · exact Or.inr <| Or.inl h
-  · exact (Or.inr ∘ Or.inr ∘ Or.inl) h
+  · grind
+  · grind
   · rcases h_insertUnit_fold (i, false) h1 with h_insertUnit_fold | h_insertUnit_fold
-    · apply Or.inr ∘ Or.inr ∘ Or.inr ∘ Exists.intro i ∘ Or.inl
-      exact ⟨h_insertUnit_fold, h2⟩
+    · grind
     · apply Or.inl ∘ Exists.intro i ∘ Or.inl
       exact ⟨h_insertUnit_fold, h2⟩
   · rcases h_insertUnit_fold (i, true) h1 with h_insertUnit_fold | h_insertUnit_fold
-    · apply Or.inr ∘ Or.inr ∘ Or.inr ∘ Exists.intro i ∘ Or.inr
-      exact ⟨h_insertUnit_fold, h2⟩
+    · grind
     · apply Or.inl ∘ Exists.intro i ∘ Or.inr
       exact ⟨h_insertUnit_fold, h2⟩
 
 theorem deleteOne_preserves_rupUnits {n : Nat} (f : DefaultFormula n) (id : Nat) :
     (deleteOne f id).rupUnits = f.rupUnits := by
   simp only [deleteOne]
-  split <;> simp only
+  grind
 
 theorem deleteOne_preserves_assignments_size {n : Nat} (f : DefaultFormula n) (id : Nat) :
     (deleteOne f id).assignments.size = f.assignments.size := by
   simp only [deleteOne]
-  split <;> simp only [Array.size_modify]
+  grind
 
 theorem deleteOne_preserves_strongAssignmentsInvariant {n : Nat} (f : DefaultFormula n) (id : Nat) :
     StrongAssignmentsInvariant f → StrongAssignmentsInvariant (deleteOne f id) := by
@@ -466,11 +423,7 @@ theorem deleteOne_preserves_strongAssignmentsInvariant {n : Nat} (f : DefaultFor
       by_cases l.1.1 = i.1
       · next l_eq_i =>
         simp only [l_eq_i, Array.getElem_modify_self] at hb
-        have l_ne_b : l.2 ≠ b := by
-          intro l_eq_b
-          rw [← l_eq_b] at hb
-          have hb' := not_has_remove f.assignments[i.1] l.2
-          simp [hb] at hb'
+        have l_ne_b : l.2 ≠ b := by grind [not_has_remove]
         replace l_ne_b := Bool.eq_not_of_ne l_ne_b
         simp only [l_ne_b] at hb
         have hb := has_remove_irrelevant f.assignments[i.1] b hb
@@ -519,23 +472,19 @@ theorem deleteOne_preserves_strongAssignmentsInvariant {n : Nat} (f : DefaultFor
           · rcases List.getElem_of_mem hf with ⟨idx, hbound, hidx⟩
             simp only [← hidx, Array.toList_set]
             rw [List.mem_iff_get]
-            have idx_in_bounds : idx < List.length (List.set f.clauses.toList id none) := by
-              simp only [List.length_set]
-              exact hbound
+            have idx_in_bounds : idx < List.length (List.set f.clauses.toList id none) := by grind
             apply Exists.intro ⟨idx, idx_in_bounds⟩
             by_cases id = idx
             · next id_eq_idx =>
               exfalso
-              have idx_in_bounds2 : idx < f.clauses.size := by
-                conv => rhs; rw [List.size_toArray]
-                exact hbound
+              have idx_in_bounds2 : idx < f.clauses.size := by grind
               simp only [id_eq_idx, getElem!_def, idx_in_bounds2, Array.getElem?_eq_getElem, ←
                 Array.getElem_toList] at heq
               rw [hidx, hl] at heq
               simp only [unit, Option.some.injEq, DefaultClause.mk.injEq, List.cons.injEq, and_true] at heq
               have i_eq_l : i = l.1 := by rw [← heq]
               simp only [i_eq_l, not_true] at l_ne_i
-            · next id_ne_idx => simp [id_ne_idx]
+            · next id_ne_idx => grind
           · exact hf
         · exact Or.inr hf
     · simp only [Prod.exists, Bool.exists_bool, not_exists, not_or, unit] at hl
@@ -547,25 +496,10 @@ theorem deleteOne_preserves_strongAssignmentsInvariant {n : Nat} (f : DefaultFor
         rw [heq] at hl
         specialize hl l.1
         simp only [DefaultClause.mk.injEq, List.cons.injEq, and_true] at hl
-        by_cases hl2 : l.2
-        · simp only [← hl2, not_true, and_false] at hl
-        · simp only [Bool.not_eq_true] at hl2
-          simp only [← hl2, not_true, false_and] at hl
+        by_cases hl2 : l.2 <;> grind
       · have deleteOne_f_rw : deleteOne f id = ⟨Array.set! f.clauses id none, f.rupUnits, f.ratUnits, f.assignments⟩ := by
           simp only [deleteOne]
-          split
-          · next heq2 =>
-            simp [heq] at heq2
-          · next l _ _ heq2 =>
-            simp only [heq, Option.some.injEq] at heq2
-            rw [heq2] at hl
-            specialize hl l.1
-            simp only [DefaultClause.mk.injEq, List.cons.injEq, and_true] at hl
-            by_cases hl2 : l.2
-            · simp only [← hl2, not_true, and_false] at hl
-            · simp only [Bool.not_eq_true] at hl2
-              simp only [← hl2, not_true, false_and] at hl
-          · rfl
+          grind
         simp only [deleteOne_f_rw] at hb
         specialize hf i b hb
         simp only [toList, List.append_assoc, List.mem_append, List.mem_filterMap, id_eq,
@@ -580,25 +514,15 @@ theorem deleteOne_preserves_strongAssignmentsInvariant {n : Nat} (f : DefaultFor
             simp only [← hidx, Array.toList_set]
             rw [List.mem_iff_get]
             have idx_in_bounds : idx < List.length (List.set f.clauses.toList id none) := by
-              simp only [List.length_set]
-              exact hbound
+              grind
             apply Exists.intro ⟨idx, idx_in_bounds⟩
             by_cases id = idx
             · next id_eq_idx =>
               exfalso
-              have idx_in_bounds2 : idx < f.clauses.size := by
-                conv => rhs; rw [List.size_toArray]
-                exact hbound
-              simp only [id_eq_idx, getElem!_def, idx_in_bounds2, Array.getElem?_eq_getElem, ←
-                Array.getElem_toList] at heq
-              rw [hidx] at heq
-              simp only [Option.some.injEq] at heq
-              rw [← heq] at hl
-              specialize hl i
-              simp only [unit, DefaultClause.mk.injEq, List.cons.injEq, Prod.mk.injEq, true_and, and_true,
-                Bool.not_eq_false, Bool.not_eq_true] at hl
-              by_cases b_val : b <;> simp [b_val] at hl
-            · next id_ne_idx => simp [id_ne_idx]
+              have idx_in_bounds2 : idx < f.clauses.size := by grind
+              simp only [id_eq_idx, getElem!_def, idx_in_bounds2] at heq
+              grind [unit]
+            · next id_ne_idx => grind
           · exact hf
         · exact Or.inr hf
 
@@ -611,25 +535,23 @@ theorem readyForRupAdd_delete {n : Nat} (f : DefaultFormula n) (arr : Array Nat)
     have hl (acc : DefaultFormula n) (ih : acc.rupUnits = #[]) (id : Nat) (_id_in_arr : id ∈ arr.toList) :
       (deleteOne acc id).rupUnits = #[] := by rw [deleteOne_preserves_rupUnits, ih]
     exact List.foldlRecOn arr.toList deleteOne hb hl
-  · have hb : StrongAssignmentsInvariant f := h.2
-    have hl (acc : DefaultFormula n) (ih : StrongAssignmentsInvariant acc) (id : Nat) (_id_in_arr : id ∈ arr.toList) :
+  · have hl (acc : DefaultFormula n) (ih : StrongAssignmentsInvariant acc) (id : Nat) (_id_in_arr : id ∈ arr.toList) :
       StrongAssignmentsInvariant (deleteOne acc id) := deleteOne_preserves_strongAssignmentsInvariant acc id ih
-    exact List.foldlRecOn arr.toList deleteOne hb hl
+    exact List.foldlRecOn arr.toList deleteOne h.2 hl
 
 theorem deleteOne_preserves_ratUnits {n : Nat} (f : DefaultFormula n) (id : Nat) :
     (deleteOne f id).ratUnits = f.ratUnits := by
   simp only [deleteOne]
-  split <;> simp only
+  grind
 
 theorem readyForRatAdd_delete {n : Nat} (f : DefaultFormula n) (arr : Array Nat) :
     ReadyForRatAdd f → ReadyForRatAdd (delete f arr) := by
   intro h
   constructor
   · rw [delete, ← Array.foldl_toList]
-    have hb : f.ratUnits = #[] := h.1
     have hl (acc : DefaultFormula n) (ih : acc.ratUnits = #[]) (id : Nat) (_id_in_arr : id ∈ arr.toList) :
-      (deleteOne acc id).ratUnits = #[] := by rw [deleteOne_preserves_ratUnits, ih]
-    exact List.foldlRecOn arr.toList deleteOne hb hl
+      (deleteOne acc id).ratUnits = #[] := by grind [deleteOne_preserves_ratUnits]
+    exact List.foldlRecOn arr.toList deleteOne h.1 hl
   · exact readyForRupAdd_delete f arr h.2
 
 theorem deleteOne_subset (f : DefaultFormula n) (id : Nat) (c : DefaultClause n) :
@@ -645,25 +567,16 @@ theorem deleteOne_subset (f : DefaultFormula n) (id : Nat) (c : DefaultClause n)
       simp only [List.mem_filterMap, id_eq, exists_eq_right] at h1
       simp only [List.mem_filterMap, id_eq, exists_eq_right]
       rw [Array.set!, Array.setIfInBounds] at h1
-      split at h1
-      · simp only [Array.toList_set] at h1
-        rcases List.getElem_of_mem h1 with ⟨i, h, h4⟩
-        rw [List.getElem_set] at h4
-        split at h4
-        · simp at h4
-        · rw [← h4]
-          apply List.getElem_mem
-      · exact h1
-    · exact (Or.inr ∘ Or.inl) h1
-    · exact (Or.inr ∘ Or.inr) h1
+      grind
+    · grind
+    · grind
 
 theorem delete_subset (f : DefaultFormula n) (arr : Array Nat) (c : DefaultClause n) :
     c ∈ toList (delete f arr) → c ∈ toList f := by
   simp only [delete, ← Array.foldl_toList]
-  have hb : c ∈ toList f → c ∈ toList f := id
   have hl (f' : DefaultFormula n) (ih : c ∈ toList f' → c ∈ toList f) (id : Nat) (_ : id ∈ arr.toList) :
-    c ∈ toList (deleteOne f' id) → c ∈ toList f := by intro h; exact ih <| deleteOne_subset f' id c h
-  exact List.foldlRecOn arr.toList deleteOne hb hl
+    c ∈ toList (deleteOne f' id) → c ∈ toList f := by grind [deleteOne_subset]
+  exact List.foldlRecOn arr.toList deleteOne id hl
 
 end DefaultFormula
 
